\documentclass{article}
%=============================================================================80
%	                          Packages                                     %
%==============================================================================%
% Packages
\usepackage[utf8]{inputenc}
\usepackage{graphicx}
\usepackage{amsmath}
\usepackage{amssymb}
\usepackage{braket}
\usepackage{float}
\usepackage{subcaption}
\usepackage{nicefrac}
\usepackage[margin=0.7in]{geometry}
\usepackage[version=4]{mhchem}
%==============================================================================%
%                           User-Defined Commands                              %
%==============================================================================%
% User-Defined Commands
\newcommand{\be}{\begin{equation}}
\newcommand{\ee}{\end{equation}}
\newcommand{\benum}{\begin{enumerate}}
\newcommand{\eenum}{\end{enumerate}}
\newcommand{\pd}{\partial}
\newcommand{\dg}{\dagger}
\newcommand{\half}{\frac{1}{2}}
\newcommand{\nhalf}{\nicefrac{1}{2}}
\newcommand{\pri}{\frac{\pd}{\pd r_i}}
\newcommand{\bM}{\mbox{\bf M}}
\newcommand{\bS}{\mbox{\bf S}}
\newcommand{\bK}{\mbox{\bf K}}
\newcommand{\br}{\mbox{\bf r}}
\newcommand{\bp}{\mbox{\bf p}}
%==============================================================================%
%                             Title Information                                %
%==============================================================================%
\title{Chem237: Lecture 16}
\date{5/10/18}
\author{Shane Flynn}
%==============================================================================%
\begin{document}

\maketitle

\section{Note}
I have just transcribed the lecture notes, no thought has gone in yet. We need to sit down and analyze this. 9-15-19

\section{Normal Mode Analysis; Quantum Case}
We begin by writing the Hamiltonian for our system of interest with N vibrational degrees of freedom,
\be
\begin{split}
    \widehat{H}&= \sum_{i = 1}^{N} \frac{-1}{2 m}  \frac{\pd^2}{\pd r_i^2}+ V(r_1,\dots,r_N)\\
    &=-\half \nabla^T\bM^{-1}\nabla + \half \br^T\bK\br
\end{split}
\ee
Where $\nabla$ refers to a set of partial derivitives $\nabla = \pri$.


We will begin by mass-scaling our coordinates (no momentum).
\be
\begin{split}
    \br' &:= \bM^{\nhalf}\br\\
    \nabla' &:= \bM^{-\nhalf}\nabla =
    \begin{bmatrix}
        \frac{1}{\sqrt{m_1}} \pri\\
        \vdots \\
        \frac{1}{\sqrt{m_N}} \pri
    \end{bmatrix}\\
    \bK' &:= \bM^{-\nhalf}\bK \bM^{-\nhalf}
\end{split}
\ee

In our new coordinates the Hamiltonian reads
\be
    \widehat{H}= -\half\nabla'^T\nabla+\half\br'^T\bK'\br'
\ee
Which is analagous to the classical case.

Normal mode analysis is useful for chemistry and physics problems, for example the simple harmonic oscillator.
%==============================================================================
% Vlad gave up on going over the example after drawing it but it's a very commonly used example so I know what the solution should be.
% This is the first time I solved it using the method Vlad taught.
%==============================================================================
\subsection{Example}
Consider an example of two classical masses attached to three springs as shown in the figure below.
%==============================================================================
 % Somebody should make a figure that looks like the drawing Vlad made in class
 % It's the same as the one in this website:
 % http://scienceworld.wolfram.com/physics/SpringsThreeSpringsandTwoMasses.html
%==============================================================================
The Hamiltonian for the system is simple to write because we just have coupled harmonic oscillators.
\be
  H = \frac{p_1^2}{2 m_1} + \frac{p_2^2}{2 m_2} + \frac{k_1}{2}r_1^2 + \frac{k_2}{2}(r_1 - r_2)^2 + \frac{k_3}{2}r_2^2
\ee
For simplicity, let's just say that the spring constants are the same, i.e. $k_1 = k_2 = k_3 = k$, and the masses are the same, i.e. $m_1 = m_2 = m$.
So now our Hamiltonian simplifies to,
\be
  \begin{split}
    H &= \frac{p_1^2}{2 m} + \frac{p_2^2}{2 m} + \frac{k}{2}r_1^2 + \frac{k}{2}(r_1 - r_2)^2 + \frac{k}{2}r_2^2 \\
    &= \frac{1}{2m} \Big( p_1^2 + p_2^2 \Big) + \frac{k}{2} \Big( 2r_1^2 - 2r_1 r_2 + 2r_2^2 \Big)
  \end{split}
\ee
where $r_1$ and $r_2$ are each mass's coordinates measured from the equilibrium position.
By creating mass, coordinate, momenta, and Hessian matrices, we can make this look like equation (\ref{eq:gen_hamil}),
\be
\begin{split}
  \textbf{H} &= \frac{1}{2} \bp^T \bM^{-1} \bp + \frac{1}{2} \textbf{r}^{T} \bK \textbf{r} \\
  &= \frac{1}{2}
  \begin{bmatrix}
    p_1 \\
    p_2 \\
  \end{bmatrix}^T
  \begin{bmatrix}
    m & 0 \\
    0 & m \\
  \end{bmatrix}^{-1}
  \begin{bmatrix}
    p_1 \\
    p_2 \\
  \end{bmatrix}
   + \frac{1}{2}
   \begin{bmatrix}
     r_1 \\
     r_2 \\
   \end{bmatrix}^T
   \begin{bmatrix}
     2k & -k \\
     -k & 2k \\
   \end{bmatrix}
   \begin{bmatrix}
     r_1 \\
     r_2 \\
   \end{bmatrix}
 \end{split}
\ee
The mass matrix is simply a diagonal matrix because there are no cross terms in the kinetic energy.
However, the cross terms in the Hessian come from the $(r_1 - r_2)^2$ term in the potential.
If you're not sure where each matrix element came from, recall equation (8),
\be
  K_{i j} = \frac{\partial^2 V}{\partial r_i r_j} .
\ee
Since the potential is equal to,
\be
  V = \frac{k}{2} \Big( 2r_1^2 - 2r_1 r_2 + 2r_2^2 \Big)
\ee
we can say that the matrix elements for the Hessian are,
\be
  K_{11} = \frac{\partial^2 V}{\partial r_1^2} = 2k \quad ; \quad K_{12} =  \frac{\partial^2 V}{\partial r_1 r_2} = K_{21} = -k \quad ; \quad K_{22} = \frac{\partial^2 V}{\partial r_2^2} = 2k .
\ee
You can verify that equation 15 and 16 are the same.

Now we can define the mass-scaled Hessian,
\be
  \bK' =
  \begin{bmatrix}
    \frac{2 k}{\sqrt{m_1^2}} & - \frac{k}{\sqrt{m_1 m_2}} \\
    - \frac{k}{\sqrt{m_1 m_2}} & \frac{2k}{\sqrt{m_2^2}} \\
  \end{bmatrix}
  =
  \begin{bmatrix}
    \frac{2 k}{m} & - \frac{k}{m} \\
    - \frac{k}{m} & \frac{2k}{m} \\
  \end{bmatrix}
\ee
and find it's eigenvalues and eigenvectors. This can be easily done with Mathematica, but we can also do this by hand since our system is 2 dimensional. To find the eigenvalues, we set up the characteristic equation,
\be
  \text{det}(\bK' - \lambda \textbf{I}) = 0 \Longrightarrow \Big(\frac{2k}{m} - \lambda \Big)^2 - \Big( \frac{k}{m} \Big)^2 = 0 \Longrightarrow \Big( \lambda - \frac{2k}{m} \Big)^2 - \Big( \frac{k}{m} \Big)^2 = 0
\ee
and solve for $\lambda$.
\be
  \begin{split}
  \lambda - \frac{2k}{m} =& \pm \frac{k}{m} \Longrightarrow \lambda = \frac{2k}{m} \pm \frac{k}{m} \\
  &\lambda_1 = \frac{3k}{m} , \lambda_2 = \frac{k}{m}
  \end{split}
\ee
Now we find the eigenvector for each eigenvalue.

For $\lambda_1$, we have
\be
  \bK' \textbf{x} = \lambda_1 \textbf{x} \Longrightarrow (\bK' - \lambda_1 \textbf{I}) \textbf{x} = \textbf{0} \Longrightarrow
  \begin{bmatrix}
    \frac{2k}{m} - \lambda_1 & \frac{-k}{m} \\
    \frac{-k}{m} & \frac{2k}{m} - \lambda_1 \\
  \end{bmatrix}
  \begin{bmatrix}
    x_1 \\
    x_2 \\
  \end{bmatrix}
  =
  \begin{bmatrix}
    0 \\
    0 \\
  \end{bmatrix}
\ee
which is just solving two equations with two unknowns.
\be
  \begin{split}
    \frac{-k}{m}x_1 - \frac{k}{m}x_2 &= 0 \\
    \frac{-k}{m}x_1 - \frac{k}{m}x_2 &= 0 \\
  \end{split}
\ee
Since both equations are the same, we are really only left with one equation and two unknowns. To get around the problem, we can assign any value to $x_1$, like $x_1 = 1$, and just solve for $x_2$.
\be
  \frac{-k}{m}(1) - \frac{k}{m}x_2 = 0 \Longrightarrow x_2 = -1
\ee
So our eigenvector for $\lambda_1$ is $\begin{bmatrix} 1 \\ -1 \\ \end{bmatrix}$. If you don't understand why I was able to do this, refer to Lecture 14.

For $\lambda_2$, we have
\be
  \bK' \textbf{x} = \lambda_2 \textbf{x} \Longrightarrow (\bK' - \lambda_2 \textbf{I}) \textbf{x} = \textbf{0} \Longrightarrow
  \begin{bmatrix}
    \frac{2k}{m} - \lambda_2 & \frac{-k}{m} \\
    \frac{-k}{m} & \frac{2k}{m} - \lambda_2 \\
  \end{bmatrix}
  \begin{bmatrix}
    x_1 \\
    x_2 \\
  \end{bmatrix}
  =
  \begin{bmatrix}
    0 \\
    0 \\
  \end{bmatrix} .
\ee
So our two equations are:
\be
  \begin{split}
    \frac{k}{m}x_1 - \frac{k}{m}x_2 &= 0 \\
    \frac{-k}{m}x_1 + \frac{k}{m}x_2 &= 0 \\
  \end{split}
\ee
The bottom equation is just the top equation multiplied by $-1$. To solve this, we again assign $x_1 = 1$ and solve for $x_2$.
\be
  \frac{k}{m}(1) - \frac{k}{m}x_2 \Longrightarrow x_2 = 1
\ee
So our eigenvector for $\lambda_2$ is $\begin{bmatrix} 1 \\ 1 \\ \end{bmatrix}$. The eigendecomposition equation for the mass-scaled Hessian becomes,
\be
  \bK' = \textbf{U} \Lambda \textbf{U}^{\dagger} =
  \begin{bmatrix}
    -1 & 1 \\
    1 & 1 \\
  \end{bmatrix}
  \begin{bmatrix}
    \frac{3k}{m} & 0 \\
    0 & \frac{k}{m} \\
  \end{bmatrix}
  \begin{bmatrix}
    -1 & 1 \\
    1 & 1 \\
  \end{bmatrix}^{\dagger} .
\ee
Remember that each column of \textbf{U} is the ith eigenvector that corresponds to the ith eigenvalue.

The normal mode coordinates and momenta are then defined from the mass-scaled coordinates and momenta.
\be \label{eq:ex_sol}
  \begin{split}
    \tilde{\br} &= \textbf{U}^{\dagger} \br' =
    \begin{bmatrix}
      -1 & 1 \\
      1 & 1 \\
    \end{bmatrix}^{\dagger}
    \begin{bmatrix}
      \sqrt{m} r_1 \\
      \sqrt{m} r_2 \\
    \end{bmatrix}
    =
    \begin{bmatrix}
       \sqrt{m} (r_2 - r_1) \\
       \sqrt{m} (r_1 + r_2) \\
    \end{bmatrix}
    =
    \begin{bmatrix}
      \tilde{r}_1 \\
      \tilde{r}_2 \\
    \end{bmatrix}
    = \sqrt{m}
    \begin{bmatrix}
        (r_2 - r_1) \\
        (r_1 + r_2) \\
    \end{bmatrix}
    \\
    \tilde{\bp} &= \textbf{U}^{\dagger} \bp'
    \begin{bmatrix}
      -1 & 1 \\
      1 & 1 \\
    \end{bmatrix}^{\dagger}
    \begin{bmatrix}
      \frac{1}{\sqrt{m}} p_1 \\
      \frac{1}{\sqrt{m}} p_2 \\
    \end{bmatrix}
    =
    \begin{bmatrix}
      \frac{1}{\sqrt{m}} (p_2 - p_1) \\
      \frac{1}{\sqrt{m}} (p_1 + p_2) \\
    \end{bmatrix}
    =
    \begin{bmatrix}
      \tilde{p}_1 \\
      \tilde{p}_2 \\
    \end{bmatrix}
    =
    \frac{1}{\sqrt{m}}
    \begin{bmatrix}
     (p_2 - p_1) \\
     (p_1 + p_2) \\
    \end{bmatrix}
  \end{split}
\ee
And with this, we have effectively turned our original coupled system into a system of independent harmonic oscillators!
In other words, in the normal mode basis, we can think of our system as having 2 normal modes: one where both masses oscillate with frequency $\omega_1 = \sqrt{\frac{3k}{m}}$ and another where both masses oscillate with frequency $\omega_2 = \sqrt{\frac{k}{m}}$.
Also, the position and momenta of both masses in each normal mode can be described with $(\tilde{r_1},\tilde{p_1})$ and $(\tilde{r_2},\tilde{p_2})$.

You may wonder why the position and momenta do not look sinusoidal. This is because we never explicitly defined $r_1$ and $r_2$. However, we expect both masses to osciallte sinusoidally so we can assume that the solutions will be sinusoidal.


\subsection{Explicit 3D Example}
For another example, consider a 3D Potential,
\be
\begin{split}
V(x,y,z):&= \left(x-y\right)^2 + \left(x+y\right)^2 + \left(z-x\right)^2\\
&= 3x^2+2y^2+z^2-2xz .
\end{split}
\ee

The forces are given by
\be
  F(x,y,z) = -\nabla V(x,y,z) =
  \begin{bmatrix}
    \left(-\frac{\pd V}{\pd x}\right)_{y,z}\\
    \left(-\frac{\pd V}{\pd y}\right)_{x,z}\\
    \left(-\frac{\pd V}{\pd z}\right)_{x,y}
  \end{bmatrix}
  = \begin{bmatrix}
    -2(3x-z) \\
    -4y  \\
    -2(z-x) \\
  \end{bmatrix}
\ee

And the associated Hessian,
\be
\bK = \begin{bmatrix}
\frac{\pd^2 V}{\pd x^2} & \frac{\pd^2 V}{\pd x\pd y} &\frac{\pd^2 V}{\pd x\pd z} \\
\frac{\pd^2 V}{\pd y\pd x} & \frac{\pd^2 V}{\pd y^2} &\frac{\pd^2 V}{\pd y\pd z} \\
\frac{\pd^2 V}{\pd z\pd x} & \frac{\pd^2 V}{\pd z \pd y} &\frac{\pd^2 V}{\pd z^2} \\
\end{bmatrix} = \begin{bmatrix}
6 & 0 & -2\\
0 & 4 & 0\\
-2 & 0 & 2\\
\end{bmatrix}
\ee

The problem can be simplified if we consider the Hamiltonian,
\be
\begin{split}
\widehat{H}&= \widehat{T} + \widehat{V} \\
&= \frac{P_x^2}{2m_1}+\frac{P_y^2}{2m_2}+\frac{P_z^2}{2m_3}+3x^2+2y^2+z^2-2xz\\
&= \left( \frac{P_y^2}{2m_2}+2y^2 \right) + \left( \frac{P_x^2}{2m_1}+\frac{P_z^2}{2m_3}+3x^2+z^2-2xz \right)\\
&= H_y + H_{xz}
\end{split}
\ee
with $H_y:=\frac{P_y^2}{2m_2}+2y^2$ and $H_{xz}:=
\frac{P_x^2}{2m_1}+\frac{P_z^2}{2m_3}+3x^2+z^2-2xz$.
We can see that $H_y$ is just a 1D Quantum Harmonic Oscillator which has a well-known solution,
\be
E_y = \hbar \omega_y\left(n_y+\half\right)\;\bigg|\; \omega_y=\left(\frac{k_y}{m_2}\right)^{\nhalf} .
\ee
where $k_y=4$.

We can decouple the degrees of freedom in $H_{xy}$ using normal modes.
The hessian associated with this 2D system is,
\be
\bK = \begin{bmatrix}
\frac{\pd^2 V}{\pd x^2} &\frac{\pd^2 V}{\pd x\pd z} \\
\frac{\pd^2 V}{\pd z\pd x} & \frac{\pd^2 V}{\pd z^2} \\
\end{bmatrix} = \begin{bmatrix}
6 & -2\\
-2 & 2\\
\end{bmatrix}
\ee
For convenience let the masses all be equal $m_1=m_2=m_3=m$, so the mass-scaled
Hessian ($\bK'$) then reads
\be
\bK'= \begin{bmatrix}
\frac{6}{m} & -\frac{2}{m}\\
-\frac{2}{m} & \frac{2}{m}
\end{bmatrix}
\ee
The normal modes are determined from solving the eigenvalue problem.
\be
\det\left(\bK' - \lambda \textbf{I} \right)=
\begin{bmatrix}
\frac{6}{m}-\lambda & -\frac{2}{m}\\
-\frac{2}{m} & \frac{2}{m}-\lambda
\end{bmatrix} = \left(\frac{6}{m}-\lambda\right) \left(\frac{2}{m}-\lambda\right) - \frac{4}{m^2} = 0
\ee
The subsequent eigenvalues give us the normal mode frequencies.
\be
\begin{split}
\lambda^2-\frac{8}{m} \lambda + \frac{8}{m^2} &= 0 \\
\lambda_1&=\frac{4 + 2 \sqrt{2}}{m}\\
\lambda_2&=\frac{4 - 2 \sqrt{2}}{m}\\
\end{split}
\ee
So the energy $E_{xz}$ can be written as a sum of the normal mode energies.
\be
E_{xz} = \hbar \left( \frac{4 + 2 \sqrt{2}}{m} \right) \left( n_x + \half \right) + \hbar \left( \frac{4 - 2 \sqrt{2}}{m} \right) \left( n_z + \half \right)
\ee
Therefore the analytic expression for our enery is given by the sum of the energies, $E_{x,y,z} = E_y + E_{xz}$.
\be
E_{x,y,z} = \hbar\left[\left(\frac{4}{m}\right)^{\nhalf} \left(n_y+\half \right) +
\frac{4 + 2 \sqrt{2}}{m}\left(n_x+\half\right) + \frac{4 - 2 \sqrt{2}}{m}\left(n_z+\half\right) \right]
\ee
where $n_i=0,1,2,\dots$

\section{Normal Mode Analysis of Time Signals}
A time signal is simply data as a function of time (c(t)), an important tdata type for most experiments,
andis usualy a set of discrete measurements made in time.
A standard analysis of time signals is to describte c(t) as a sum of expotnetials.
\be\label{eq:time}
c(t) = \sum_{k=1}^K d_k e^{-\lambda_kt}
\ee

Where c(t) is know data and d, $\lambda$ are unknown parameters.
The central numerical problem then is to fit a signal to a expotentials.

time analysis data is usualy a set of N discrete measurements made in time.
\be
c(t) \Rightarrow c(n\tau) = \sum_{n=0}^{N-1} c_n
\ee

A nieve approach would be to use a non-linear least square optimization.
You can define an optimizaiton function F in terms of our parameters.
\be
F(\lambda_k,d_k) := \sum_{n=1}^{N-1}\left( c_n - \sum_{k=1}^K d_k e^{-\lambda_kn\tau}  \right)^2
\ee
And there are tons of variations for taking this approach.

I fyou can exactly fit your data the actual form of the fitting function is not important, normally there is no exact solution .

N is the numer of data points in teh experiment, k is the number of expotentials to use int eh fitting process, usually N $>>$ k, so you have an overdetermined problem.
This means you are trying to find the best solution, which therefore epend s on the function you use to minimize (F).
This means we are really trying to minimize F itself, we have an optimization problem to minimize F.
\be
\text{min}_{\lambda_k,d_k}\; F(\lambda_k,d_k)
\ee

If you have a non-linear function F, it will typically have many minima and typically the global minimum is the best fit.
Unfortunately teh number of minima grows with the size of the space, $\approx e^{\alpha k}$.
roughly speaking with about 10 parameters global optimizaiton becomes very dificult numerically.

Although eq. \ref{eq:time} looks bad is is actually a special case (Proxy 1793 maybe discovered).

Disconnected you could solve this problem using linear algebra, find the roots of a polynomial degree k.

convex optimizationL function is a special case where the function of parameters only has 1 minimum.

\subsection{General Problem}
The problem is generalized to complex space as

\be
\begin{split}
    c_n &= \sum_{k=1}^K d_k e^{-in\tau \omega_k}\\
    d_k &= |d_k|e^{i\theta}\\
    \omega_k &= V_k - i\lambda_k
\end{split}
\ee
Here ($d_k,\omega_k \in \mathbb{C}$)

So the general problem actually has expotential decay.
\be
e^{-in\tau \omega_k} = e^{in\tau V_k}e^{-n\tau \lambda_k}
\ee
%%%%%%%%%%%%%%%%%%%%%%%%%%%%%%%%%%%%%%%%%%%%%%%%%%%%%%%%%%%%%%%%%%%%%%
%Insert a graph plotting this expotnetial it will oscilate with smaller and smaller amplitude
%%%%%%%%%%%%%%%%%%%%%%%%%%%%%%%%%%%%%%%%%%%%%%%%%%%%%%%%%%%%%%%%%%%%%%
In the complex case we have 2 complex numbers that are unknowns.
$c_n \in mathbb{C}, d_k, \omega \in \mathbb{C}$.
This is a well know problem, one approach to solve is the Harmonic Inversion.
Here the goal is to invert the time signal with a sum of harmonic contributions.
Hamonic inversion is related to spectra estimation methods.

We need to formulate the linear algebra problem to solve for frequency and amplitude.
Spectral analysis: given $c_n = c(n\tau)$ estimate the spectra (I is our estimate).
\be
I(\omega) := \int_0^\infty dt\; c(t)\; e^{i\omega t}
\ee

Here we have a finite interval (finite set of data measurements) and we want to estimate the result to infinity.
\be
\begin{split}
    I(\omega) &\approx \tau \sum_{n=1}^\infty c(n\tau)e^{i\omega\tau}\\
    &= \tau \sum_{n=0}^\infty c_n z^{-n}
\end{split}
\ee
Where we define ($z:=e^{-i\omega\tau}$).

Can we try an estimate our infinite series from the finite measurement?
\be
I(\omega) \approx \sum_{n=i}^{N-1} c_n z^{-n}
\ee

This is valid, however, it converges very slowly.
Also a larger problem is known as the fourier transform ncertainty principle, where resolution is given by $\delta \omega \approx \frac{1}{\alpha} N$.

In principle if N$\geq$ 2k then you can solve the problem exactly.
So the paramaterization fir problem can circumvent the Fourier Transform uncertainty principle and get better resolution.

let $U_k = e^{-i\tau\omega_k}$
\be
\begin{split}
    &\sum_{n=0}^\infty c_nz^{-n}\\
    c_n &= \sum_{k=1}^K d_k U_k^n\\
    &= \sum_{n=0}^\infty \sum_{k=1}^K d_k\left(\frac{U_k}{z}\right)^n\\
    &= \sum_{k=1}^K \sum_{n=0}^\infty d_k\left(\frac{U_k}{z}\right)^n\\
    &= \sum_{k=1}^K \sum_{n=0}^\infty d_k\left(\frac{U_k}{z}\right)^n\\
    &= \sum_{k=1}^K d_k \sum_{n=0}^\infty \left(\frac{U_k}{z}\right)^n\\
    &= \sum_{k=1}^K d_k \; \frac{1}{1 - \frac{\omega_k}{z}}
\end{split}
\ee
Where $\sum_{n=0}^\infty \left(\frac{U_k}{z}\right)^n$ is a geometric series.
With $d_k,omega_k$ parameters you can solve.

Some approximations, $\omega_k = V_k - i\lambda_k$ , but $\lambda_k$ is usually small, if $\tau$ is small than
\be
\frac{1}{1-\frac{\omega_k}{z}} = \frac{1}{1-e^{i(\omega-\omega_k)\tau}} \approx \frac{1}{i(\omega_k-\omega)\tau}
\ee

\be
\begin{split}
    \frac{1}{\omega-\omega_k} &= \frac{1}{(\omega-\omega_k)+i\lambda_k} \\
    &= \frac{\omega-V_k}{(\omega-V_k)^2 + \lambda_k^2} - i \frac{\lambda_k}{(\omega-V_k)^2+\lambda_k^2}
\end{split}
\ee

The last two terms are a complex lorentzian function.
%%%%%%%%%%%5talk abotu whateve this funciton is

The first term is the absorption (small $\lambda_k$ corresponds to a narrow peak).
%plot first term, and entire thing

so if our oscillations can be dscribed by $e^{-in\tau\omega_k}$ you get a complex lorentzian function.

So how do we solv this problem
\be
c_n = \sum_{k=1}^K d_kU_k^n
\ee
Where we have k=1,K unknown parameters and ($d_k,U_k \in \mathbb{C}$), given c$_n$?

\subsection{Vlad Solutoin}
There are many different ways to solve this problem.
One solution (vlads old paper, Neuhauser 1995?) assumes the known data can be represented as
\be
c_n := \theta^T\widehat{U}^N\theta
\ee

Where $\widehat{U}$ is a symmetric linear operator (a symmetric matrix $\in \mathbb{C}$), not hermitian and $\theta$ is a column vector.

This assumption is a special case for time signals.
It is consistent witht he time auto correlatio nfunction for a quantum system.
\be
\Psi(t) = e^{-it\widehat{H}} \Psi(0) = \widehat{U}^n\phi
\ee
If we define ($\phi:= \Psi(0), \; U:= e^{-it\widehat{H}}$).

With these definition the time autocorrelation function becomes
\be
\braket{\Psi(t)|\Psi(0)} = \phi^T\widehat{U}^N\phi
\ee
Which is exactly our $c_n$.
So the time signal is represented by some quantum system with quantum autocoreelation funciton given by some operator.

\subsection{Analysis}
We now have a quantum system, so lets solve the eigenvalue problem (U our eigenvalues and $\gamma$ our eigenvectors).
\be
\begin{split}
    \widehat{U}\gamma_k&=U_k\gamma\\
    \widehat{U}&=\sum_kU_k\gamma_k\gamma_k^T\\
\end{split}
\ee

These two statements are equivalent, this is known as the eigenrepresentation of an operator, it is equivalent to eigendecomposition.
%We need ot explain this proof better.
We know that $\widehat{U}$ is symmetric i.e. $\widehat{U}=\widehat{U}^T$ therefore the right/left eigenvetors are the same i.e. ($\gamma_k^T\gamma_k=\delta_{kl}$), meaning the eigenvectors are orthogonal for symmetric matricies.
\be
\left( \sum_k U_k\gamma_k\gamma_k^T \right) \gamma_l = U_l\gamma_l
\ee
So we see this is simply an eigenvector equivalent to the eigenvalue problem.

If we let $(\gamma_k^T\phi)^2 = \phi^T\gamma_k \gamma_k^T\phi \equiv d_k$ we have
\be
c_n = \phi^T\widehat{U}^N\phi = \sum_k \phi^T U_N^N \gamma_k\gamma_k^T\phi = \sum_k d_kU_k^N
\ee

Where we used the operator as a fucntion of a matrix ($\widehat{U}^N = \sum_k U_k^N\gamma_k\gamma_K^T$)

So our time signal is defined by U and d, using $c_N=\phi^T\widehat{U}^N\phi$ reduces teh parameter estimation problem to an eigenvalue problme.

Now we can solve the eigenvalue problem.
\be
\widehat{U}\gamma_k = U_k\gamma_k
\ee
We don't actually want any of these terms explicitly, we know c (the data) and we assume $c_N=\phi^T\widehat{U}^N\phi$ , we don't want to find expressions for any of the other terms.

In QM we define a basis and evaluate the hamiltonian matrix to solve.
So we need to express our matrix elements in terms of c.

We define our basis to be
\be
\begin{split}
    \phi_n &:= \widehat{U}\phi\\
    \phi_0 &= \phi\\
    \phi_1 &= \widehat{U}\phi_0\\
    \phi_2 &= \widehat{U}\phi_1\\
    &\;\;\vdots
\end{split}
\ee

This basis choice i similar to a Krylov basis (super matricies).
You simply keep multiplying to get the Kryloc vectors, genearating a Krylov subspace, using these vectors you can understand the original matrix of interest.

We will use this basis to find the operator $\widehat{U}$, and therefore solve the generalized eigevalue problem.
\be
\begin{split}
    U_{nm} &= \phi^T\widehat{U}\phi\\
    \delta_{nm} &= \phi^T_n\phi_m\\
    (U-U_k \bS)B_k&= 0
\end{split}
\ee
Where U and delta are square matricies of size M by M.
\be
\delta_{nk} = \phi_N^T\phi_m = (\widehat{U}^n\phi)^T(U^m\phi)
\ee
$\widehat{U}$ is symmetric therefore
\be
\delta_{nk} = \phi^T\widehat{U}^{n+m}\phi = c_{m+n}
\ee
Where $c_{m+n}$ is our data.
Overlap matrix is computed with teh data points directly.

\be
U_{nm} = \phi^T\widehat{U}\phi_m = c_{n+m+1}
\ee

U and S are matricies we get from our data, meaning we can solve the eigenvalue problem $(U-U_k \bS)B_k= 0$.

It can be shwon that $(\gamma_k^T\phi)^2 = d_k$ so we assume
\be
\gamma_k = \sum_{n=1}^{m-1} B_{kn}\phi_n
\ee
Wxpanding the eigenfunctions nto the basis function leads to
%need to show this somehow
\be
d_k = \left[\sum_{n=0}^{m-1}\left(B_{kn}c_n\right)\right]^2
\ee

So we solve the generalized eigenvalue problem with dtaa matricies and find $U_k, d_k$.

\end{document}
